\section{Conservation of stress-energy}

Conservation of stress energy implies the following equations
\begin{equation}
\nabla_a T^{ab} = \nabla_a p^{ab} + u^b \nabla_a \rho u^a + \rho u^a \nabla_a u^b.
\end{equation}
The contraction with the four-velocity in particular yields the following equation
\begin{equation}
u_b\nabla_ap^{ab} = \nabla_a \rho u^a
\end{equation}
and differentiating the expression $u_bp^{ab}$ gives
\begin{equation}
-p^{ab}\nabla_au_b = \nabla_a \rho u^a.
\end{equation}
This can now be expanded
\begin{eqnarray}
-\frac{p^{ab}\nabla_au_b}{n} = -\tau^{ab}\nabla_au_b & = &  \frac{\nabla_a n\epsilon u^a}{n} = u^a \nabla_a \epsilon +  \frac{\epsilon}{n}\nabla_a nu^a = u^a \nabla_a \epsilon \\
-\tau^{ab}\nabla_au_b & = &  u^a \frac{\partial \epsilon}{\partial H^{BC}}\frac{\partial H^{BC}}{\partial x^a} = u^a\frac{\tau_{BC}}{2}\frac{\partial }{\partial x^a} g^{bc}f^B{}_bf^C{}_c \\
& = &u^a\frac{\tau_{BC}}{2} \left( g^{bc}{}_{,a}f^B{}_bf^C{}_c  + g^{bc}f^B{}_{ab}f^C{}_c + g^{bc}f^B{}_bf^C{}_{ac}\right).
\end{eqnarray}
Now, since $u^af^A{}_a = 0$, $u^a{}_{,b}f^A{}_a = - u^af^A{}_{ab}$ and
\begin{eqnarray}
-\tau^{ab}\nabla_au_b & = &  \frac{\tau_{BC}}{2} \left( u^a g^{bc}{}_{,a}f^B{}_bf^C{}_c  - u^a{}_{,b}g^{bc}f^B{}_af^C{}_c - u^a{}_{,c}g^{bc}f^B{}_bf^C{}_a\right) \\
& = &  u^a g^{bc}{}_{,a}\frac{\tau_{bc}}{2}  - u^a{}_{,b}g^{bc}\frac{\tau_{ac}}{2} - u^a{}_{,c}g^{bc}\frac{\tau_{ab}}{2} = u^{a'} g^{b'c'}{}_{,a'}\frac{\tau_{b'c'}}{2}  - u^a{}_{,b'}g^{b'c'}\frac{\tau_{ac'}}{2} - u^a{}_{,c}g^{bc}\frac{\tau_{ab}}{2} \\
& = & u^{c} g^{ab}{}_{,c}\frac{\tau_{ab}}{2}  - u^a{}_{,c}g^{cb}\frac{\tau_{ab}}{2} - u^a{}_{,c}g^{bc}\frac{\tau_{ab}}{2} = \frac{\tau^{a'b'}}{2} g_{aa'}g_{bb'}\left( u^{c} g^{ab}{}_{,c}  - 2u^a{}_{,c}g^{cb}\right).
\end{eqnarray}
Substituting $u^a{}_{,c} = \nabla_c u^a - \Gamma^a_{cd}u^d$
\begin{eqnarray}
-\tau^{ab}\nabla_au_b & = & \frac{\tau^{a'b'}}{2} g_{aa'}g_{bb'}\left( u^{c} g^{ab}{}_{,c}  - 2g^{cb} \nabla_c u^a + 2\Gamma^a_{cd}u^dg^{cb}\right) \\
 & = & -\tau^{a'b'} \nabla_{b'} u_{a'} + \frac{\tau^{a'b'}}{2}\left( 2\Gamma_{a'b'd}u^d + g_{aa'}g_{bb'}u^cg^{ab}{}_{,c} \right).
\end{eqnarray}
Using properties of the Levi-Civita connection $\nabla_c g^{ab} = g^{ab}{}_{,c} + \Gamma^a_{cd}g^{bd} + \Gamma^b_{cd}g^{ad}$ and
\begin{eqnarray}
-\tau^{ab}\nabla_au_b & = & -\tau^{a'b'} \nabla_{b'} u_{a'} + \frac{\tau^{a'b'}}{2}\left( 2\Gamma_{a'b'd}u^d - g_{aa'}g_{bb'}u^c(\Gamma^a_{cd}g^{bd} + \Gamma^b_{cd}g^{ad}) \right)\\
& = & -\tau^{ab} \nabla_{b} u_{a} + \frac{\tau^{a'b'}}{2}\left( 2\Gamma_{a'b'd}u^d - u^c \Gamma_{a'cb'} - u^c\Gamma_{b'ca'} \right)\\
& = & -\tau^{ab} \nabla_{b} u_{a} + \frac{\tau^{ab}}{2}u^c\left( \Gamma_{abc} - \Gamma_{bac} \right)\\
& = & -\tau^{ab} \nabla_{b} u_{a},
\end{eqnarray}
where the last propertry follows from contracting a symmetric tensor with an anti-symmetric one. This equation is therefore trivially satisfied by virtue of the definition of the pressure tensor.

It turns out to be simpler to deal with the divergence of the mixed
stress energy tensor
\begin{equation}
\nabla_a T^a{}_b = \nabla_a\left( p^a{}_b + \rho u^au_b \right) =
\nabla_a p^a{}_b + u_b\nabla_a\rho u^a + \rho u^a\nabla_a u_b = 0.
\end{equation}
These remaining conservation laws may be simplified by substituting $\nabla_a \rho u^a = u_c \nabla_ap^{ac}$ so that
\begin{equation}
\left(\delta_b^c + u_bu^c\right) \nabla_a p^a{}_c + \rho u^a \nabla_a
u_b = 0
\end{equation}
for $i=1\dots 3$ so long as the slicing is time-like. Expanding the covariant derivatives
\begin{equation}
\left(\delta_b^c + u_bu^c\right) \left(\partial_a p^a{}_c +
\Gamma^a_{ad}p^d{}_c - \Gamma^d_{ac}p^a{}_d\right) + \rho u^a
\left(\partial_a u_b - \Gamma^c_{ab}u_c\right).
\end{equation}
This completes the description of the equations of motion, as derived from stress-energy conservation.
